libcrux-ml-dsa/src/simd/avx2/encoding/commitment.rs
@@ -2,66 +2,6 @@ use libcrux_intrinsics::avx2::*;
 
 use minicore::abstractions::{bit::Bit, bitvec::BitVec};
 
-fn pointwise(x: BitVec<128>) -> BitVec<128> {
-    macro_rules! mk_match {
-        ($i:ident $x:ident $($l:literal)*) => {
-            match $i {
-                $($l => $x[$l],)*
-                _ => unreachable!(),
-            }
-        }
-    }
-    BitVec::from_fn(|i| {
-        mk_match!(i x   0 1 2 3 4 5 6 7 8 9 10 11 12 13 14 15 16 17 18 19 20 21 22 23 24 25 26 27 28 29 30 
-                        31 32 33 34 35 36 37 38 39 40 41 42 43 44 45 46 47 48 49 50 51 52 53 54 55 56 57 58
-                        59 60 61 62 63 64 65 66 67 68 69 70 71 72 73 74 75 76 77 78 79 80 81 82 83 84 85 86
-                        87 88 89 90 91 92 93 94 95 96 97 98 99 100 101 102 103 104 105 106 107 108 109 110 111
-                        112 113 114 115 116 117 118 119 120 121 122 123 124 125 126 127)
-    })
-}
-
-#[hax_lib::fstar::before(r#"
-let rw (x: Minicore.Abstractions.Bitvec.t_BitVec (mk_u64 128)): Lemma (x == pointwise x) = admit ()
-
-[@@FStar.Tactics.V2.(postprocess_with (fun () -> 
-        let done = alloc false in
-        ctrl_rewrite TopDown (fun _ -> if read done then (false, Skip) else (true, Continue))
-                             (fun _ -> (fun () -> apply_lemma_rw (`rw); write done true)
-                                       `or_else` trefl);
-        norm [primops; iota; delta_namespace ["Core"; "Libcrux_ml_dsa"; "Libcrux_intrinsics"; "Minicore"; "FStar.FunctionalExtensionality"; "Rust_primitives"]; zeta_full];
-        compute ();
-        norm [primops; iota; delta; zeta_full]
-        ))]
-"#)]
-fn serialize_4_aux(simd_unit: &Vec256) -> Vec128 {
-    let adjacent_2_combined = mm256_sllv_epi32_u32(*simd_unit, 0, 28, 0, 28, 0, 28, 0, 28);
-    let x = adjacent_2_combined;
-    let adjacent_2_combined = mm256_srli_epi64::<28>(adjacent_2_combined);
-
-    let adjacent_4_combined =
-        mm256_permutevar8x32_epi32_u32(adjacent_2_combined, 0, 0, 0, 0, 6, 2, 4, 0);
-    let adjacent_4_combined = mm256_castsi256_si128(adjacent_4_combined);
-    mm_shuffle_epi8_u8(
-        adjacent_4_combined,
-        0xF0,
-        0xF0,
-        0xF0,
-        0xF0,
-        0xF0,
-        0xF0,
-        0xF0,
-        0xF0,
-        0xF0,
-        0xF0,
-        0xF0,
-        0xF0,
-        12,
-        4,
-        8,
-        0,
-    )
-}
-
 #[hax_lib::ensures(|r| {
     use hax_lib::*;
     let r = BitVec::<128>::from(r);
@@ -70,65 +10,52 @@ fn serialize_4_aux(simd_unit: &Vec256) -> Vec128 {
         implies(i < 32, r[i] == simd_unit[i / 4 * 32 + i % 4])
     )
 })]
+#[inline(always)]
 fn serialize_4(simd_unit: &Vec256) -> Vec128 {
-    serialize_4_aux(simd_unit)
+    #[hax_lib::fstar::before(r#"
+    [@@FStar.Tactics.V2.(postprocess_with (fun () -> 
+            let done = alloc false in
+            ctrl_rewrite TopDown (fun _ -> if read done then (false, Skip) else (true, Continue))
+                                 (fun _ -> (fun () -> apply_lemma_rw (`${BitVec::<128>::rewrite_pointwise}); write done true)
+                                           `or_else` trefl);
+            let crate = match cur_module () with | crate::_ -> crate | _ -> fail "Empty module name" in
+            norm [primops; iota; delta_namespace ["Core"; crate; "Libcrux_intrinsics"; "Minicore"; "FStar.FunctionalExtensionality"; "Rust_primitives"]; zeta_full];
+            compute ();
+            norm [primops; iota; delta; zeta_full];
+            trefl ()
+            ))]
+    "#)]
+    #[inline(always)]
+    fn aux(simd_unit: Vec256) -> Vec128 {
+        let adjacent_2_combined = mm256_sllv_epi32_u32(simd_unit, 0, 28, 0, 28, 0, 28, 0, 28);
+        let x = adjacent_2_combined;
+        let adjacent_2_combined = mm256_srli_epi64::<28>(adjacent_2_combined);
+
+        let adjacent_4_combined =
+            mm256_permutevar8x32_epi32_u32(adjacent_2_combined, 0, 0, 0, 0, 6, 2, 4, 0);
+        let adjacent_4_combined = mm256_castsi256_si128(adjacent_4_combined);
+        mm_shuffle_epi8_u8(
+            adjacent_4_combined,
+            0xF0,
+            0xF0,
+            0xF0,
+            0xF0,
+            0xF0,
+            0xF0,
+            0xF0,
+            0xF0,
+            0xF0,
+            0xF0,
+            0xF0,
+            0xF0,
+            12,
+            4,
+            8,
+            0,
+        )
+    }
+    aux(*simd_unit)
 }
-
-// mod spec {
-//     use minicore::arch::x86::{extra::*, *};
-
-//     pub fn serialize_4(simd_unit: &__m256i, out: &mut [u8]) -> __m256i {
-//         let mut serialized = [0u8; 19];
-//         debug_assert!(out.len() == 4);
-
-//         let adjacent_2_combined = mm256_sllv_epi32_u32(*simd_unit, 0, 28, 0, 28, 0, 28, 0, 28);
-//         let x = adjacent_2_combined;
-//         let adjacent_2_combined = _mm256_srli_epi64::<28>(adjacent_2_combined);
-
-//         let adjacent_4_combined =
-//             mm256_permutevar8x32_epi32_u32(adjacent_2_combined, 0, 0, 0, 0, 6, 2, 4, 0);
-//         let adjacent_4_combined = _mm256_castsi256_si128(adjacent_4_combined);
-//         let adjacent_4_combined = mm_shuffle_epi8_u8(
-//             adjacent_4_combined,
-//             0xF0,
-//             0xF0,
-//             0xF0,
-//             0xF0,
-//             0xF0,
-//             0xF0,
-//             0xF0,
-//             0xF0,
-//             0xF0,
-//             0xF0,
-//             0xF0,
-//             0xF0,
-//             12,
-//             4,
-//             8,
-//             0,
-//         );
-
-//         mm_storeu_bytes_si128(&mut serialized[0..16], adjacent_4_combined);
-
-//         out.copy_from_slice(&serialized[0..4]);
-
-//         x
-//     }
-// }
-
-// #[test]
-// fn test_4() {
-//     use minicore::abstractions::bitvec::BitVec;
-//     for _ in 0..1000 {
-//         let vector: BitVec<256> = BitVec::rand();
-//         let mut out_l = [0u8; 4];
-//         let mut out_r = [0u8; 4];
-//         let l = serialize_4(&vector.into(), &mut out_l);
-//         let r = spec::serialize_4(&vector, &mut out_r);
-//         assert_eq!(BitVec::from(l), r);
-//         assert_eq!(out_l, out_r);
-//     }
-// }
 
 #[inline(always)]
 pub(in crate::simd::avx2) fn serialize(simd_unit: &Vec256, out: &mut [u8]) {
@@ -136,25 +63,7 @@ pub(in crate::simd::avx2) fn serialize(simd_unit: &Vec256, out: &mut [u8]) {
 
     match out.len() as u8 {
         4 => {
-            let adjacent_2_combined =
-                mm256_sllv_epi32(*simd_unit, mm256_set_epi32(0, 28, 0, 28, 0, 28, 0, 28));
-            let adjacent_2_combined = mm256_srli_epi64::<28>(adjacent_2_combined);
-
-            let adjacent_4_combined = mm256_permutevar8x32_epi32(
-                adjacent_2_combined,
-                mm256_set_epi32(0, 0, 0, 0, 6, 2, 4, 0),
-            );
-            let adjacent_4_combined = mm256_castsi256_si128(adjacent_4_combined);
-            let adjacent_4_combined = mm_shuffle_epi8(
-                adjacent_4_combined,
-                mm_set_epi8(
-                    0xF0, 0xF0, 0xF0, 0xF0, 0xF0, 0xF0, 0xF0, 0xF0, 0xF0, 0xF0, 0xF0, 0xF0, 12, 4,
-                    8, 0,
-                ),
-            );
-
-            mm_storeu_bytes_si128(&mut serialized[0..16], adjacent_4_combined);
-
+            mm_storeu_bytes_si128(&mut serialized[0..16], serialize_4(simd_unit));
             out.copy_from_slice(&serialized[0..4]);
         }
 
