libcrux-ml-dsa/proofs/fstar/extraction/Libcrux_ml_dsa.Simd.Avx2.Encoding.Commitment.fst
@@ -3,161 +3,13 @@ module Libcrux_ml_dsa.Simd.Avx2.Encoding.Commitment
 open Core
 open FStar.Mul
 
-let _ =
-  (* This module has implicit dependencies, here we make them explicit. *)
-  (* The implicit dependencies arise from typeclasses instances. *)
-  let open Minicore.Abstractions.Bitvec in
-  ()
-
-let pointwise (x: Minicore.Abstractions.Bitvec.t_BitVec (mk_u64 128)) =
-  Minicore.Abstractions.Bitvec.impl_7__from_fn (mk_u64 128)
-    (fun i ->
-        let i:u64 = i in
-        match i <: u64 with
-        | Rust_primitives.Integers.MkInt 0 -> x.[ mk_u64 0 ] <: Minicore.Abstractions.Bit.t_Bit
-        | Rust_primitives.Integers.MkInt 1 -> x.[ mk_u64 1 ] <: Minicore.Abstractions.Bit.t_Bit
-        | Rust_primitives.Integers.MkInt 2 -> x.[ mk_u64 2 ] <: Minicore.Abstractions.Bit.t_Bit
-        | Rust_primitives.Integers.MkInt 3 -> x.[ mk_u64 3 ] <: Minicore.Abstractions.Bit.t_Bit
-        | Rust_primitives.Integers.MkInt 4 -> x.[ mk_u64 4 ] <: Minicore.Abstractions.Bit.t_Bit
-        | Rust_primitives.Integers.MkInt 5 -> x.[ mk_u64 5 ] <: Minicore.Abstractions.Bit.t_Bit
-        | Rust_primitives.Integers.MkInt 6 -> x.[ mk_u64 6 ] <: Minicore.Abstractions.Bit.t_Bit
-        | Rust_primitives.Integers.MkInt 7 -> x.[ mk_u64 7 ] <: Minicore.Abstractions.Bit.t_Bit
-        | Rust_primitives.Integers.MkInt 8 -> x.[ mk_u64 8 ] <: Minicore.Abstractions.Bit.t_Bit
-        | Rust_primitives.Integers.MkInt 9 -> x.[ mk_u64 9 ] <: Minicore.Abstractions.Bit.t_Bit
-        | Rust_primitives.Integers.MkInt 10 -> x.[ mk_u64 10 ] <: Minicore.Abstractions.Bit.t_Bit
-        | Rust_primitives.Integers.MkInt 11 -> x.[ mk_u64 11 ] <: Minicore.Abstractions.Bit.t_Bit
-        | Rust_primitives.Integers.MkInt 12 -> x.[ mk_u64 12 ] <: Minicore.Abstractions.Bit.t_Bit
-        | Rust_primitives.Integers.MkInt 13 -> x.[ mk_u64 13 ] <: Minicore.Abstractions.Bit.t_Bit
-        | Rust_primitives.Integers.MkInt 14 -> x.[ mk_u64 14 ] <: Minicore.Abstractions.Bit.t_Bit
-        | Rust_primitives.Integers.MkInt 15 -> x.[ mk_u64 15 ] <: Minicore.Abstractions.Bit.t_Bit
-        | Rust_primitives.Integers.MkInt 16 -> x.[ mk_u64 16 ] <: Minicore.Abstractions.Bit.t_Bit
-        | Rust_primitives.Integers.MkInt 17 -> x.[ mk_u64 17 ] <: Minicore.Abstractions.Bit.t_Bit
-        | Rust_primitives.Integers.MkInt 18 -> x.[ mk_u64 18 ] <: Minicore.Abstractions.Bit.t_Bit
-        | Rust_primitives.Integers.MkInt 19 -> x.[ mk_u64 19 ] <: Minicore.Abstractions.Bit.t_Bit
-        | Rust_primitives.Integers.MkInt 20 -> x.[ mk_u64 20 ] <: Minicore.Abstractions.Bit.t_Bit
-        | Rust_primitives.Integers.MkInt 21 -> x.[ mk_u64 21 ] <: Minicore.Abstractions.Bit.t_Bit
-        | Rust_primitives.Integers.MkInt 22 -> x.[ mk_u64 22 ] <: Minicore.Abstractions.Bit.t_Bit
-        | Rust_primitives.Integers.MkInt 23 -> x.[ mk_u64 23 ] <: Minicore.Abstractions.Bit.t_Bit
-        | Rust_primitives.Integers.MkInt 24 -> x.[ mk_u64 24 ] <: Minicore.Abstractions.Bit.t_Bit
-        | Rust_primitives.Integers.MkInt 25 -> x.[ mk_u64 25 ] <: Minicore.Abstractions.Bit.t_Bit
-        | Rust_primitives.Integers.MkInt 26 -> x.[ mk_u64 26 ] <: Minicore.Abstractions.Bit.t_Bit
-        | Rust_primitives.Integers.MkInt 27 -> x.[ mk_u64 27 ] <: Minicore.Abstractions.Bit.t_Bit
-        | Rust_primitives.Integers.MkInt 28 -> x.[ mk_u64 28 ] <: Minicore.Abstractions.Bit.t_Bit
-        | Rust_primitives.Integers.MkInt 29 -> x.[ mk_u64 29 ] <: Minicore.Abstractions.Bit.t_Bit
-        | Rust_primitives.Integers.MkInt 30 -> x.[ mk_u64 30 ] <: Minicore.Abstractions.Bit.t_Bit
-        | Rust_primitives.Integers.MkInt 31 -> x.[ mk_u64 31 ] <: Minicore.Abstractions.Bit.t_Bit
-        | Rust_primitives.Integers.MkInt 32 -> x.[ mk_u64 32 ] <: Minicore.Abstractions.Bit.t_Bit
-        | Rust_primitives.Integers.MkInt 33 -> x.[ mk_u64 33 ] <: Minicore.Abstractions.Bit.t_Bit
-        | Rust_primitives.Integers.MkInt 34 -> x.[ mk_u64 34 ] <: Minicore.Abstractions.Bit.t_Bit
-        | Rust_primitives.Integers.MkInt 35 -> x.[ mk_u64 35 ] <: Minicore.Abstractions.Bit.t_Bit
-        | Rust_primitives.Integers.MkInt 36 -> x.[ mk_u64 36 ] <: Minicore.Abstractions.Bit.t_Bit
-        | Rust_primitives.Integers.MkInt 37 -> x.[ mk_u64 37 ] <: Minicore.Abstractions.Bit.t_Bit
-        | Rust_primitives.Integers.MkInt 38 -> x.[ mk_u64 38 ] <: Minicore.Abstractions.Bit.t_Bit
-        | Rust_primitives.Integers.MkInt 39 -> x.[ mk_u64 39 ] <: Minicore.Abstractions.Bit.t_Bit
-        | Rust_primitives.Integers.MkInt 40 -> x.[ mk_u64 40 ] <: Minicore.Abstractions.Bit.t_Bit
-        | Rust_primitives.Integers.MkInt 41 -> x.[ mk_u64 41 ] <: Minicore.Abstractions.Bit.t_Bit
-        | Rust_primitives.Integers.MkInt 42 -> x.[ mk_u64 42 ] <: Minicore.Abstractions.Bit.t_Bit
-        | Rust_primitives.Integers.MkInt 43 -> x.[ mk_u64 43 ] <: Minicore.Abstractions.Bit.t_Bit
-        | Rust_primitives.Integers.MkInt 44 -> x.[ mk_u64 44 ] <: Minicore.Abstractions.Bit.t_Bit
-        | Rust_primitives.Integers.MkInt 45 -> x.[ mk_u64 45 ] <: Minicore.Abstractions.Bit.t_Bit
-        | Rust_primitives.Integers.MkInt 46 -> x.[ mk_u64 46 ] <: Minicore.Abstractions.Bit.t_Bit
-        | Rust_primitives.Integers.MkInt 47 -> x.[ mk_u64 47 ] <: Minicore.Abstractions.Bit.t_Bit
-        | Rust_primitives.Integers.MkInt 48 -> x.[ mk_u64 48 ] <: Minicore.Abstractions.Bit.t_Bit
-        | Rust_primitives.Integers.MkInt 49 -> x.[ mk_u64 49 ] <: Minicore.Abstractions.Bit.t_Bit
-        | Rust_primitives.Integers.MkInt 50 -> x.[ mk_u64 50 ] <: Minicore.Abstractions.Bit.t_Bit
-        | Rust_primitives.Integers.MkInt 51 -> x.[ mk_u64 51 ] <: Minicore.Abstractions.Bit.t_Bit
-        | Rust_primitives.Integers.MkInt 52 -> x.[ mk_u64 52 ] <: Minicore.Abstractions.Bit.t_Bit
-        | Rust_primitives.Integers.MkInt 53 -> x.[ mk_u64 53 ] <: Minicore.Abstractions.Bit.t_Bit
-        | Rust_primitives.Integers.MkInt 54 -> x.[ mk_u64 54 ] <: Minicore.Abstractions.Bit.t_Bit
-        | Rust_primitives.Integers.MkInt 55 -> x.[ mk_u64 55 ] <: Minicore.Abstractions.Bit.t_Bit
-        | Rust_primitives.Integers.MkInt 56 -> x.[ mk_u64 56 ] <: Minicore.Abstractions.Bit.t_Bit
-        | Rust_primitives.Integers.MkInt 57 -> x.[ mk_u64 57 ] <: Minicore.Abstractions.Bit.t_Bit
-        | Rust_primitives.Integers.MkInt 58 -> x.[ mk_u64 58 ] <: Minicore.Abstractions.Bit.t_Bit
-        | Rust_primitives.Integers.MkInt 59 -> x.[ mk_u64 59 ] <: Minicore.Abstractions.Bit.t_Bit
-        | Rust_primitives.Integers.MkInt 60 -> x.[ mk_u64 60 ] <: Minicore.Abstractions.Bit.t_Bit
-        | Rust_primitives.Integers.MkInt 61 -> x.[ mk_u64 61 ] <: Minicore.Abstractions.Bit.t_Bit
-        | Rust_primitives.Integers.MkInt 62 -> x.[ mk_u64 62 ] <: Minicore.Abstractions.Bit.t_Bit
-        | Rust_primitives.Integers.MkInt 63 -> x.[ mk_u64 63 ] <: Minicore.Abstractions.Bit.t_Bit
-        | Rust_primitives.Integers.MkInt 64 -> x.[ mk_u64 64 ] <: Minicore.Abstractions.Bit.t_Bit
-        | Rust_primitives.Integers.MkInt 65 -> x.[ mk_u64 65 ] <: Minicore.Abstractions.Bit.t_Bit
-        | Rust_primitives.Integers.MkInt 66 -> x.[ mk_u64 66 ] <: Minicore.Abstractions.Bit.t_Bit
-        | Rust_primitives.Integers.MkInt 67 -> x.[ mk_u64 67 ] <: Minicore.Abstractions.Bit.t_Bit
-        | Rust_primitives.Integers.MkInt 68 -> x.[ mk_u64 68 ] <: Minicore.Abstractions.Bit.t_Bit
-        | Rust_primitives.Integers.MkInt 69 -> x.[ mk_u64 69 ] <: Minicore.Abstractions.Bit.t_Bit
-        | Rust_primitives.Integers.MkInt 70 -> x.[ mk_u64 70 ] <: Minicore.Abstractions.Bit.t_Bit
-        | Rust_primitives.Integers.MkInt 71 -> x.[ mk_u64 71 ] <: Minicore.Abstractions.Bit.t_Bit
-        | Rust_primitives.Integers.MkInt 72 -> x.[ mk_u64 72 ] <: Minicore.Abstractions.Bit.t_Bit
-        | Rust_primitives.Integers.MkInt 73 -> x.[ mk_u64 73 ] <: Minicore.Abstractions.Bit.t_Bit
-        | Rust_primitives.Integers.MkInt 74 -> x.[ mk_u64 74 ] <: Minicore.Abstractions.Bit.t_Bit
-        | Rust_primitives.Integers.MkInt 75 -> x.[ mk_u64 75 ] <: Minicore.Abstractions.Bit.t_Bit
-        | Rust_primitives.Integers.MkInt 76 -> x.[ mk_u64 76 ] <: Minicore.Abstractions.Bit.t_Bit
-        | Rust_primitives.Integers.MkInt 77 -> x.[ mk_u64 77 ] <: Minicore.Abstractions.Bit.t_Bit
-        | Rust_primitives.Integers.MkInt 78 -> x.[ mk_u64 78 ] <: Minicore.Abstractions.Bit.t_Bit
-        | Rust_primitives.Integers.MkInt 79 -> x.[ mk_u64 79 ] <: Minicore.Abstractions.Bit.t_Bit
-        | Rust_primitives.Integers.MkInt 80 -> x.[ mk_u64 80 ] <: Minicore.Abstractions.Bit.t_Bit
-        | Rust_primitives.Integers.MkInt 81 -> x.[ mk_u64 81 ] <: Minicore.Abstractions.Bit.t_Bit
-        | Rust_primitives.Integers.MkInt 82 -> x.[ mk_u64 82 ] <: Minicore.Abstractions.Bit.t_Bit
-        | Rust_primitives.Integers.MkInt 83 -> x.[ mk_u64 83 ] <: Minicore.Abstractions.Bit.t_Bit
-        | Rust_primitives.Integers.MkInt 84 -> x.[ mk_u64 84 ] <: Minicore.Abstractions.Bit.t_Bit
-        | Rust_primitives.Integers.MkInt 85 -> x.[ mk_u64 85 ] <: Minicore.Abstractions.Bit.t_Bit
-        | Rust_primitives.Integers.MkInt 86 -> x.[ mk_u64 86 ] <: Minicore.Abstractions.Bit.t_Bit
-        | Rust_primitives.Integers.MkInt 87 -> x.[ mk_u64 87 ] <: Minicore.Abstractions.Bit.t_Bit
-        | Rust_primitives.Integers.MkInt 88 -> x.[ mk_u64 88 ] <: Minicore.Abstractions.Bit.t_Bit
-        | Rust_primitives.Integers.MkInt 89 -> x.[ mk_u64 89 ] <: Minicore.Abstractions.Bit.t_Bit
-        | Rust_primitives.Integers.MkInt 90 -> x.[ mk_u64 90 ] <: Minicore.Abstractions.Bit.t_Bit
-        | Rust_primitives.Integers.MkInt 91 -> x.[ mk_u64 91 ] <: Minicore.Abstractions.Bit.t_Bit
-        | Rust_primitives.Integers.MkInt 92 -> x.[ mk_u64 92 ] <: Minicore.Abstractions.Bit.t_Bit
-        | Rust_primitives.Integers.MkInt 93 -> x.[ mk_u64 93 ] <: Minicore.Abstractions.Bit.t_Bit
-        | Rust_primitives.Integers.MkInt 94 -> x.[ mk_u64 94 ] <: Minicore.Abstractions.Bit.t_Bit
-        | Rust_primitives.Integers.MkInt 95 -> x.[ mk_u64 95 ] <: Minicore.Abstractions.Bit.t_Bit
-        | Rust_primitives.Integers.MkInt 96 -> x.[ mk_u64 96 ] <: Minicore.Abstractions.Bit.t_Bit
-        | Rust_primitives.Integers.MkInt 97 -> x.[ mk_u64 97 ] <: Minicore.Abstractions.Bit.t_Bit
-        | Rust_primitives.Integers.MkInt 98 -> x.[ mk_u64 98 ] <: Minicore.Abstractions.Bit.t_Bit
-        | Rust_primitives.Integers.MkInt 99 -> x.[ mk_u64 99 ] <: Minicore.Abstractions.Bit.t_Bit
-        | Rust_primitives.Integers.MkInt 100 -> x.[ mk_u64 100 ] <: Minicore.Abstractions.Bit.t_Bit
-        | Rust_primitives.Integers.MkInt 101 -> x.[ mk_u64 101 ] <: Minicore.Abstractions.Bit.t_Bit
-        | Rust_primitives.Integers.MkInt 102 -> x.[ mk_u64 102 ] <: Minicore.Abstractions.Bit.t_Bit
-        | Rust_primitives.Integers.MkInt 103 -> x.[ mk_u64 103 ] <: Minicore.Abstractions.Bit.t_Bit
-        | Rust_primitives.Integers.MkInt 104 -> x.[ mk_u64 104 ] <: Minicore.Abstractions.Bit.t_Bit
-        | Rust_primitives.Integers.MkInt 105 -> x.[ mk_u64 105 ] <: Minicore.Abstractions.Bit.t_Bit
-        | Rust_primitives.Integers.MkInt 106 -> x.[ mk_u64 106 ] <: Minicore.Abstractions.Bit.t_Bit
-        | Rust_primitives.Integers.MkInt 107 -> x.[ mk_u64 107 ] <: Minicore.Abstractions.Bit.t_Bit
-        | Rust_primitives.Integers.MkInt 108 -> x.[ mk_u64 108 ] <: Minicore.Abstractions.Bit.t_Bit
-        | Rust_primitives.Integers.MkInt 109 -> x.[ mk_u64 109 ] <: Minicore.Abstractions.Bit.t_Bit
-        | Rust_primitives.Integers.MkInt 110 -> x.[ mk_u64 110 ] <: Minicore.Abstractions.Bit.t_Bit
-        | Rust_primitives.Integers.MkInt 111 -> x.[ mk_u64 111 ] <: Minicore.Abstractions.Bit.t_Bit
-        | Rust_primitives.Integers.MkInt 112 -> x.[ mk_u64 112 ] <: Minicore.Abstractions.Bit.t_Bit
-        | Rust_primitives.Integers.MkInt 113 -> x.[ mk_u64 113 ] <: Minicore.Abstractions.Bit.t_Bit
-        | Rust_primitives.Integers.MkInt 114 -> x.[ mk_u64 114 ] <: Minicore.Abstractions.Bit.t_Bit
-        | Rust_primitives.Integers.MkInt 115 -> x.[ mk_u64 115 ] <: Minicore.Abstractions.Bit.t_Bit
-        | Rust_primitives.Integers.MkInt 116 -> x.[ mk_u64 116 ] <: Minicore.Abstractions.Bit.t_Bit
-        | Rust_primitives.Integers.MkInt 117 -> x.[ mk_u64 117 ] <: Minicore.Abstractions.Bit.t_Bit
-        | Rust_primitives.Integers.MkInt 118 -> x.[ mk_u64 118 ] <: Minicore.Abstractions.Bit.t_Bit
-        | Rust_primitives.Integers.MkInt 119 -> x.[ mk_u64 119 ] <: Minicore.Abstractions.Bit.t_Bit
-        | Rust_primitives.Integers.MkInt 120 -> x.[ mk_u64 120 ] <: Minicore.Abstractions.Bit.t_Bit
-        | Rust_primitives.Integers.MkInt 121 -> x.[ mk_u64 121 ] <: Minicore.Abstractions.Bit.t_Bit
-        | Rust_primitives.Integers.MkInt 122 -> x.[ mk_u64 122 ] <: Minicore.Abstractions.Bit.t_Bit
-        | Rust_primitives.Integers.MkInt 123 -> x.[ mk_u64 123 ] <: Minicore.Abstractions.Bit.t_Bit
-        | Rust_primitives.Integers.MkInt 124 -> x.[ mk_u64 124 ] <: Minicore.Abstractions.Bit.t_Bit
-        | Rust_primitives.Integers.MkInt 125 -> x.[ mk_u64 125 ] <: Minicore.Abstractions.Bit.t_Bit
-        | Rust_primitives.Integers.MkInt 126 -> x.[ mk_u64 126 ] <: Minicore.Abstractions.Bit.t_Bit
-        | Rust_primitives.Integers.MkInt 127 -> x.[ mk_u64 127 ] <: Minicore.Abstractions.Bit.t_Bit
-        | _ ->
-          Rust_primitives.Hax.never_to_any (Core.Panicking.panic "internal error: entered unreachable code"
-
-              <:
-              Rust_primitives.Hax.t_Never)
-          <:
-          Minicore.Abstractions.Bit.t_Bit)
-
-let rw (x: Minicore.Abstractions.Bitvec.t_BitVec (mk_u64 128)): Lemma (x == pointwise x) = admit ()
-
 [@@FStar.Tactics.V2.(postprocess_with (fun () -> 
         let done = alloc false in
         ctrl_rewrite TopDown (fun _ -> if read done then (false, Skip) else (true, Continue))
-                             (fun _ -> (fun () -> apply_lemma_rw (`rw); write done true)
+                             (fun _ -> (fun () -> apply_lemma_rw (`Minicore.Abstractions.Bitvec.impl_7__rewrite_pointwise); write done true)
                                        `or_else` trefl);
-        norm [primops; iota; delta_namespace ["Core"; "Libcrux_ml_dsa"; "Libcrux_intrinsics"; "Minicore"; "FStar.FunctionalExtensionality"; "Rust_primitives"]; zeta_full];
+        let crate = match cur_module () with | crate::_ -> crate | _ -> fail "Empty module name" in
+        norm [primops; iota; delta_namespace ["Core"; crate; "Libcrux_intrinsics"; "Minicore"; "FStar.FunctionalExtensionality"; "Rust_primitives"]; zeta_full];
         compute ();
         norm [primops; iota; delta; zeta_full];
         trefl ()
@@ -205,46 +57,6 @@ let serialize (simd_unit: Minicore.Abstractions.Bitvec.t_BitVec (mk_u64 256)) (o
   let out, serialized:(t_Slice u8 & t_Array u8 (mk_usize 19)) =
     match cast (Core.Slice.impl__len #u8 out <: usize) <: u8 with
     | Rust_primitives.Integers.MkInt 4 ->
-      let adjacent_2_combined:Minicore.Abstractions.Bitvec.t_BitVec (mk_u64 256) =
-        Libcrux_intrinsics.Avx2_extract.mm256_sllv_epi32 simd_unit
-          (Libcrux_intrinsics.Avx2_extract.mm256_set_epi32 (mk_i32 0)
-              (mk_i32 28)
-              (mk_i32 0)
-              (mk_i32 28)
-              (mk_i32 0)
-              (mk_i32 28)
-              (mk_i32 0)
-              (mk_i32 28)
-            <:
-            Minicore.Abstractions.Bitvec.t_BitVec (mk_u64 256))
-      in
-      let adjacent_2_combined:Minicore.Abstractions.Bitvec.t_BitVec (mk_u64 256) =
-        Libcrux_intrinsics.Avx2_extract.mm256_srli_epi64 (mk_i32 28) adjacent_2_combined
-      in
-      let adjacent_4_combined:Minicore.Abstractions.Bitvec.t_BitVec (mk_u64 256) =
-        Libcrux_intrinsics.Avx2_extract.mm256_permutevar8x32_epi32 adjacent_2_combined
-          (Libcrux_intrinsics.Avx2_extract.mm256_set_epi32 (mk_i32 0)
-              (mk_i32 0)
-              (mk_i32 0)
-              (mk_i32 0)
-              (mk_i32 6)
-              (mk_i32 2)
-              (mk_i32 4)
-              (mk_i32 0)
-            <:
-            Minicore.Abstractions.Bitvec.t_BitVec (mk_u64 256))
-      in
-      let adjacent_4_combined:Minicore.Abstractions.Bitvec.t_BitVec (mk_u64 128) =
-        Libcrux_intrinsics.Avx2_extract.mm256_castsi256_si128 adjacent_4_combined
-      in
-      let adjacent_4_combined:Minicore.Abstractions.Bitvec.t_BitVec (mk_u64 128) =
-        Libcrux_intrinsics.Avx2_extract.mm_shuffle_epi8 adjacent_4_combined
-          (Libcrux_intrinsics.Avx2_extract.mm_set_epi8 (mk_u8 240) (mk_u8 240) (mk_u8 240)
-              (mk_u8 240) (mk_u8 240) (mk_u8 240) (mk_u8 240) (mk_u8 240) (mk_u8 240) (mk_u8 240)
-              (mk_u8 240) (mk_u8 240) (mk_u8 12) (mk_u8 4) (mk_u8 8) (mk_u8 0)
-            <:
-            Minicore.Abstractions.Bitvec.t_BitVec (mk_u64 128))
-      in
       let serialized:t_Array u8 (mk_usize 19) =
         Rust_primitives.Hax.Monomorphized_update_at.update_at_range serialized
           ({ Core.Ops.Range.f_start = mk_usize 0; Core.Ops.Range.f_end = mk_usize 16 }
@@ -258,7 +70,7 @@ let serialize (simd_unit: Minicore.Abstractions.Bitvec.t_BitVec (mk_u64 256)) (o
                   Core.Ops.Range.t_Range usize ]
                 <:
                 t_Slice u8)
-              adjacent_4_combined
+              (serialize_4_ simd_unit <: Minicore.Abstractions.Bitvec.t_BitVec (mk_u64 128))
             <:
             t_Slice u8)
       in
